---
{"dg-publish":true,"permalink":"/sem-3/mat-1003/module-1/inverse-converse-and-contra-positive-of-a-conditional-statement/","tags":"gardenEntry"}
---

# Inverse, Converse and Contra-Positive of a Conditional Statement
---

[[Sem 3/Mat 1003/Module 1/Predicates and Quantifiers|Predicates and Quantifiers]]

---
### Inverse
Negative of both hypothesis and conclusion
-p->-q is the inverse of p->q 

### Converse
Hypothesis and conclusion gets interchanged
q->p is the converse of p->q

### Contra-positive
Interchanging the hypothesis and conclusion of the inverse statement
-q->-p is the contra-positive of p->q

### Rule of Inference #ruleofinference
##### 1. Addition
p -> p`\/`q

##### 2. Simplification
p`/\`q->p

##### 3. Conjunction
(p)`/\`(q) -> p`/\`q

##### 4. Modus Ponens
((p->q)`/\`p)->q

##### 5. Modus Tollens
((p->q)`/\`-q)->-p

##### 6. Disjunction Syllogism
((p`\/`q)`/\`-p)->q

##### 7. Hypothetical Syllogism
((p->q)`/\`(q->r))->(p->r)

##### 8. Constructive Dilemma
((p->q)`/\`(r->s)`/\`(p`\/`r))->(q`\/`s)

##### 9. Destructive Dilemma
((p->q)`/\`(r-s)`/\`(-q`\/`-s))->(-p`\/`-r)

### Checking validity of a conclusion using rule of inference
- Rule P: A premise may be introduced at any step in the derivation
- Rule T: A rule of inference may be introduced to derive a conclusion from the previously introduced premise/premises. The conclusion derived using rule T may be intermidiate conclusion which is going to act as a premise for the next step
- Rule CP: A premise or an intermidiate conclusion can be replaced with an equivalent statement

---
[[Sem 3/Mat 1003/Module 1/Methods of Proving Theorems|Methods of Proving Theorems]]
